\text{Dadas as funções $f\left( x\right) = 2x - 3$ e $g\left(x \right) = x ^{2} - 1$, determine: $gog\left( x\right)$ } \\

\text{$f\left( x\right) = 2x - 3$ e $g\left( x\right) = x^{2} - 1$} \\

gog\left(x \right) = g\left( g \left( x\right)\right) = g\left(x^{2} - 1 \right) = \left( x^{2} - 1\right)^{2} -1 = x^{4} - 2x^{2} + 1 - 1 = x^{4} - 2x^{2} \\

\text{Passo a passo:} \Rightarrow  \left( x^{2} - 1\right)^{2} -1 = \left[\left( x^{2} - 1\right) \cdot  \left(x^{2} - 1\right) \right] \\

]\left[\left( x^{2} \cdot x^{2} -1 \cdot x^{2} -1 \cdot x^{2} + 1\right) \right] \\

\left(x^{2 + 2} -x^{2} -x^{2} + 1\right)\\

x^{4} - 2x^{2} + 1 - 1\\

x^{4} - 2x^{2} + \cancel{1} - \cancel{1}\\

x^{4} - 2x^{2}\\
